StrataGenerators/SetGen/Support.lean
@@ -87,6 +87,7 @@ theorem mem_support_pick_iff {x y : Set α} :
     a ∈ support (pick (fun () => x) (fun () => y)) ↔ a ∈ support x ∨ a ∈ support y := by
   simp [support, pick_mem_iff]
 
+
 theorem bind_congr_support {x : Set α} (h : ∀ a ∈ support x, f a = g a) :
     (x >>= f) = (x >>= g) := by
   ext b; simp only [Set.bind_def', support] at *
